Prove exists_combination_raisedSingleton
Signed-off-by: Sky Wilshaw <zeramorphic@proton.me>

ConNF/Counting/Recode.lean
@@ -5,11 +5,12 @@ import ConNF.Counting.CodingFunction
 # Recoding
 
 In this file, we show that all coding functions of level `β > γ` can be expressed in terms of a set
-of `γ`-coding functions.
+of a particular class of `γ`-coding functions, called *raised* coding functions.
 
 ## Main declarations
 
-* `ConNF.foo`: Something new.
+* `ConNF.exists_combination_raisedSingleton`: Each coding function at a level `β > γ` can be
+  expressed in terms of a set of `γ`-coding functions and a `β`-support orbit.
 -/
 
 noncomputable section
@@ -23,7 +24,7 @@ variable [Params.{u}] [Level] [CoherentData] {β γ : Λ} [LeLevel β] [LeLevel 
     (hγ : (γ : TypeIndex) < β)
 
 def Combination (x : TSet β) (S : Support β) (χs : Set (CodingFunction β)) : Prop :=
-  ∀ y : TSet γ, y ∈[hγ] x ↔ ∃ χ ∈ χs, ∃ T z, χ.rel T z ∧ S ≤ T ∧ y ∈[hγ] z
+  ∀ y : TSet γ, y ∈[hγ] x ↔ ∃ χ ∈ χs, ∃ T z, χ.rel T z ∧ S.Subsupport T ∧ y ∈[hγ] z
 
 theorem combination_unique {x₁ x₂ : TSet β} {S : Support β} {χs : Set (CodingFunction β)}
     (hx₁ : Combination hγ x₁ S χs) (hx₂ : Combination hγ x₂ S χs) :
@@ -39,11 +40,11 @@ theorem Combination.smul {x : TSet β} {S : Support β} {χs : Set (CodingFuncti
   rw [TSet.mem_smul_iff, h]
   constructor
   · rintro ⟨χ, hχ, T, z, hTz, hST, hyz⟩
-    refine ⟨χ, hχ, ρᵁ • T, ρ • z, χ.smul_rel hTz ρ, Support.smul_le_smul hST ρᵁ, ?_⟩
+    refine ⟨χ, hχ, ρᵁ • T, ρ • z, χ.smul_rel hTz ρ, Support.smul_subsupport_smul hST ρᵁ, ?_⟩
     rwa [TSet.mem_smul_iff]
   · rintro ⟨χ, hχ, T, z, hTz, hST, hyz⟩
     refine ⟨χ, hχ, ρ⁻¹ᵁ • T, ρ⁻¹ • z, χ.smul_rel hTz ρ⁻¹, ?_, ?_⟩
-    · have := Support.smul_le_smul hST ρ⁻¹ᵁ
+    · have := Support.smul_subsupport_smul hST ρ⁻¹ᵁ
       simp only [allPermForget_inv, inv_smul_smul] at this ⊢
       exact this
     · rwa [TSet.mem_smul_iff, inv_inv, allPerm_inv_sderiv, smul_inv_smul]
@@ -87,7 +88,7 @@ theorem smul_raisedRel (s : Set (CodingFunction β)) (o : SupportOrbit β)
   · rwa [Support.smul_orbit]
   · exact hx.smul hγ ρ
 
-def raised (s : Set (CodingFunction β)) (o : SupportOrbit β)
+def raisedCodingFunction (s : Set (CodingFunction β)) (o : SupportOrbit β)
     (hso : ∀ S, S.orbit = o → ∃ x, Combination hγ x S s ∧ S.Supports x) : CodingFunction β where
   rel := RaisedRel hγ s o
   rel_coinjective := raisedRel_coinjective hγ s o
@@ -132,5 +133,62 @@ theorem raisedSingleton_supports (S : Support β) (y : TSet γ) :
 
 def raisedSingleton (S : Support β) (y : TSet γ) : CodingFunction β :=
   (Tangle.mk (singleton hγ y) (S + designatedSupport y ↗ hγ) (raisedSingleton_supports hγ S y)).code
+
+theorem combination_raisedSingleton (x : TSet β) (S : Support β) (hxS : S.Supports x) :
+    Combination hγ x S (raisedSingleton hγ S '' {y | y ∈[hγ] x}) := by
+  intro y
+  constructor
+  · intro hy
+    refine ⟨raisedSingleton hγ S y, ⟨y, hy, rfl⟩, S + designatedSupport y ↗ hγ, singleton hγ y,
+        ?_, ?_, ?_⟩
+    · exact Tangle.code_rel_self _
+    · exact subsupport_add
+    · rw [typedMem_singleton_iff]
+  · rintro ⟨_, ⟨w, hw, rfl⟩, T, z, hTz, hST, hyz⟩
+    have : (raisedSingleton hγ _ _).rel (S + designatedSupport w ↗ hγ) (singleton hγ w) :=
+        Tangle.code_rel_self ⟨singleton hγ w, _, raisedSingleton_supports hγ S w⟩
+    obtain ⟨ρ, h₁, h₂⟩ := CodingFunction.exists_allPerm_of_rel hTz this
+    rw [smul_eq_iff_eq_inv_smul] at h₂
+    subst h₂
+    rw [TSet.mem_smul_iff, inv_inv, typedMem_singleton_iff] at hyz
+    subst hyz
+    have : S.Subsupport (ρᵁ • T) := h₁.symm ▸ subsupport_add
+    have := smul_eq_of_subsupport hST this
+    rw [← hxS.smul_eq_of_smul_eq this] at hw
+    rwa [Set.mem_setOf_eq, TSet.mem_smul_iff, allPerm_inv_sderiv, inv_smul_smul] at hw
+
+def RaisedSingleton : Type u :=
+  { χ : CodingFunction β // ∃ S : Support β, ∃ y : TSet γ, χ = raisedSingleton hγ S y }
+
+theorem exists_combination_raisedSingleton (χ : CodingFunction β) :
+    ∃ s : Set (RaisedSingleton hγ), ∃ o : SupportOrbit β,
+    ∃ hso : ∀ S, S.orbit = o → ∃ x, Combination hγ x S (Subtype.val '' s) ∧ S.Supports x,
+      χ = raisedCodingFunction hγ (Subtype.val '' s) o hso := by
+  obtain ⟨S, x, hχ⟩ := χ.rel_dom_nonempty
+  refine ⟨(λ y ↦ ⟨raisedSingleton hγ S y, S, y, rfl⟩) '' {y : TSet γ | y ∈[hγ] x}, S.orbit, ?_, ?_⟩
+  · intro T hT
+    rw [Support.orbit_eq_iff] at hT
+    obtain ⟨ρ, rfl⟩ := hT
+    refine ⟨ρ⁻¹ • x, ?_, ?_⟩
+    · have := (combination_raisedSingleton hγ x (ρᵁ • T) (χ.supports_of_rel hχ)).smul hγ ρ⁻¹
+      rw [allPermForget_inv, inv_smul_smul] at this
+      convert this using 1
+      ext χ'
+      constructor
+      · rintro ⟨_, ⟨y, hy, rfl⟩, rfl⟩
+        exact ⟨y, hy, rfl⟩
+      · rintro ⟨y, hy, rfl⟩
+        exact ⟨_, ⟨y, hy, rfl⟩, rfl⟩
+    · have := (χ.supports_of_rel hχ).smul ρ⁻¹
+      rwa [allPermForget_inv, inv_smul_smul] at this
+  · apply CodingFunction.ext S x hχ
+    refine ⟨S, rfl, x, ?_⟩
+    convert combination_raisedSingleton hγ x S (χ.supports_of_rel hχ) using 1
+    ext χ'
+    constructor
+    · rintro ⟨_, ⟨y, hy, rfl⟩, rfl⟩
+      exact ⟨y, hy, rfl⟩
+    · rintro ⟨y, hy, rfl⟩
+      exact ⟨_, ⟨y, hy, rfl⟩, rfl⟩
 
 end ConNF
